ImpCorrectnessTest now works

src/coq/ImpCorrectnessTest.v
@@ -2,6 +2,7 @@
 Require Import QuickChick.QuickChick.
 Import QcDefaultNotation. Open Scope qc_scope.
 Import QcDoNotation.
+Require Import QuickChick.RoseTrees.
 
 Require Import ZArith.
 Require Import String.
@@ -11,7 +12,10 @@ Require Import Sumbool.
 Require Import compcert.lib.Integers.
 
 (* Vellvm dependencies *)
-Require Import Vellvm.Ollvm_ast Vellvm.Compiler Vellvm.AstLib Vellvm.CFG Vellvm.StepSemantics Vellvm.Memory.
+Require Import Vellvm.Ollvm_ast Vellvm.CFG.
+Require Import Vellvm.StepSemantics Vellvm.Memory.
+Require Import Vellvm.Compiler.
+Require Import Vellvm.CFGProp.
 Require Import Vellvm.Classes.
 Require Import Vellvm.AstLib.
 Require Import Vellvm.DecidableEquality.
@@ -20,76 +24,62 @@ Require Import Vellvm.DecidableEquality.
 Require Import Vellvm.ImpQuickChick.
 Require Import Vellvm.OllvmQuickChick.
 Require Import Vellvm.MemoryQuickChick.
+Require Import Vellvm.CompilerQuickChick.
 
 (* Logical Foundations dependencies *)
 Require Import Vellvm.Imp Vellvm.Maps Vellvm.ImpCEvalFun.
 Open Scope list_scope.
 Require Import Program.
 
-(* Verification File *)
+(* Verification Files *)
 Require Import Vellvm.ImpCorrectness.
 
-(* Derive ArbitrarySizedSuchThat for (fun a : aexp => aevalR test_state a n). *)
 
-Inductive prefix_of {A : Type}: list A -> list A -> Prop :=
-| prefix_nil : forall l : list A, prefix_of [] l
-| prefix_cons_same : forall a l1 l2, prefix_of l1 l2 -> prefix_of (a :: l1) (a :: l2).
+(** Earlier, we considered the problem of proving algorithms (the compiler) 
+    correct, and showed that we can first test for correctness by writing a 
+    property Checker for the algorithm, and running QuickChick on it. To do 
+    this, we mirrored the implementation and developed generators, Show's, and 
+    shrinkers for the data types handled by and within the implementation.
 
-Inductive suffix_of {A : Type}: list A -> list A -> Prop :=
-| suffix_nil : forall l : list A, suffix_of l []
-| suffix_app : forall a l1 l2, suffix_of l1 l2 -> suffix_of (l1 ++ [a]) (l2 ++ [a]).
+    Now, we consider the problem of proving propositions correct, and
+    show how this can be done by interpreting propositions "operationally".
+    To do this, we similarly mirror the logic development by developing 
+    generators and property Checkers for logical definitions (e.g. inductive 
+    propositions) and theorems waiting to be proved. 
 
-Instance dec_prefix_of : forall A `{eq_dec A} (l1 l2 : list A), Decidable (prefix_of l1 l2).
-Proof.
-  intros A A_decidable.
-  induction l1 as [| a l1']; unfold Decidable.
-  - intros [| a l2']; left; constructor.
-  - intros [| b l2']; try solve [right; intros H; inversion H].
-    refine
-      (match a == b with
-       | left _ =>
-         match decide (prefix_of l1' l2') with
-         | left tail_eq => _
-         | right tail_neq => right _
-         end
-       | right head_neq => right _
-       end).
-    { subst; constructor. constructor. tauto. }
-    { intros H. apply tail_neq. inversion H; subst; auto. }
-    { intros H. apply head_neq. inversion H; subst; auto. }
-Defined.
+    To see why, consider ...
+*)
 
-Instance dec_Z_leq : forall n m : int, Decidable (n <= m)%Z.
-Proof.
-  unfold Decidable. intros n m.
-  destruct (n <=? m)%Z eqn:n_m.
-  - left; rewrite Z.leb_le in n_m; auto.
-  - right; intros H; rewrite <- Z.leb_le in H;
-      rewrite n_m in H; inversion H.
-Defined.
 
-Definition compile_aexp_monotonic_aux
-           (g : ctxt) (a : aexp) (n m : int) (code: list elt)
-  :=
+(** ** A small example *)
+
+Fixpoint prefix_bool {A : Type} `{eq_dec A} (l1 l2 : list A) :=
+  match l1, l2 with
+  | [], _ => true
+  | (x :: xs), (y :: ys) =>
+    if x == y then prefix_bool xs ys else false
+  | _, [] => false
+  end.
+
+Definition compile_aexp_monotonic_bool
+           (g : ctxt) (a : aexp) (n m : int) (code: list elt) :=
     let '((n', m', code'), v_opt) := compile_aexp g a (n,m,code) in
     match v_opt with
     | inl err => false
     | inr v' =>
       andb (andb (Z.leb n n') (Z.leb m m'))
-           (match decide (prefix_of (List.rev code) (List.rev code')) with
-            | left _ => true
-            | right _ => false
-            end)
+           (prefix_bool (List.rev code) (List.rev code'))
     end.
 
+(** Define property Checkers for lemmas and theorems. *)
 Definition test_compile_aexp_monotonic (a : aexp) (n m : int) :=
   let fvs := IDSet.elements (fv a) in
-  let g := compile_fv fvs in (* using this as initial context and code for now *)
+  let g := compile_fv fvs in (* use this as initial context and code for now *)
   let '((n', m', c), new_context_opt) := g (n, m, [])%Z in
   match new_context_opt with
   | inl e => whenFail "Compilation of free variables failed" false
   | inr new_context =>   
-    checker (compile_aexp_monotonic_aux new_context a n' m' c)
+    checker (compile_aexp_monotonic_bool new_context a n' m' c)
   end.
 
 (*! Section TestCompileAexpMonotonic *)
@@ -104,61 +94,87 @@ Definition test_compile_aexp_monotonic_wrapper :=
 Remove Hints genSaexp : typeclass_instances.
 (* End Section *)
 
-Definition bundled_memory := ((list id) * ctxt * env * memory * Imp.state)%type.
+(** ** Generators, Shows, and Functions *)
 
-Definition satisfies_memory_invariant_and_bound (m : bundled_memory) (n : int) : Prop :=
-  match m with
-  | (_, c, e, mem, s) => memory_invariant c e mem s /\ env_lt n e
-  end.
+Instance gen_iid :
+  GenSuchThat (int * instr_id)
+              (fun '(n, id) => iid n id) :=
+  {| arbitraryST :=
+       do! n <- arbitrary;
+       returnGen (Some (n, IId (lid_of_Z n)))
+  |}.
 
-Fixpoint check_env_lt (n : int) (e : env) : bool :=
-  match e with
-  | [] => true
-  | (Raw local_id, _) :: rest =>
-    if Z.ltb local_id n then check_env_lt n rest
-    else false
-  | _ => false
-  end.
+Instance gen_Rv64 `{Gen int64}: GenSuchThat (dvalue * int64) (fun '(v, i) => Rv64 v i) :=
+  {| arbitraryST :=
+       do! i <- arbitrary;
+       returnGen (Some (DVALUE_I64 i, i))
+  |}.
 
-Fixpoint check_memory_invariant (m : bundled_memory) :=
-  match m with
-  | ([], _, _, _, _) => true
-  | (Id var :: vars, c, e, mem, st) =>
-    match lookup_env e (Name var) with
-    | Some (DVALUE_Addr a) =>
-      if (List.nth_default undef mem a) == DVALUE_I64 (st (Id var)) then true
-      else false
-    | _ => false
-    end
-  end.
+Instance gen_Rv1: GenSuchThat (dvalue * bool) (fun '(v, b) => Rv1 v b) :=
+  {| arbitraryST :=
+       do! b <- arbitrary;
+     match b with
+     | true => returnGen (Some (DVALUE_I1 StepSemantics.Int1.one, b))
+     | false => returnGen (Some (DVALUE_I1 StepSemantics.Int1.zero, b))
+     end
+  |}.
 
-Definition check_memory_invariant_and_bound (m : bundled_memory) (n : int) : bool :=
-  match m with
-  | (vars, c, e, mem, s) =>
-    andb (check_memory_invariant (vars, c, e, mem, s))
-         (check_env_lt n e)
-  end.
+Instance show_bundled_memory : Show (list id * ctxt * env * memory * Imp.state) :=
+  {| show x := 
+       match x with
+       | (ids, c, e, m, s) =>
+         ("vars: " ++ (show ids) ++ "; " ++
+                   "env: " ++ (show e) ++ "; " ++
+                   "mem: " ++ (show m) ++ "; ")%string
+       end
+  |}.
 
-Definition aexp_correct_relation1
-           (vars : list id) (g : ctxt) (e: env) (st : Imp.state) 
-           (bound : int) (v : Ollvm_ast.value) (ans : int64)
-           (k : stack) (fn : function_id) (bid: block_id)
-           (phis : list (local_id * phi)) (term : (instr_id * terminator))
-           (s : SS.state) (mem : memory) :=
-  let '(pc', e', k') := s in
-  pc' = slc_pc fn bid phis term [] /\
-  satisfies_memory_invariant_and_bound (vars, g, e', mem, st) bound /\
-  Rv64e (eval_op e' (Some (TYPE_I 64)%Z) v) ans /\
-  env_extends e e'.
+(** The following deviates from the logic development in two ways. Firstly,
+    we introduce (vars : list id) so that we can compute with the domain of 
+    Imp.state; this is essential for Checking. Secondly, we generate elements
+    that satisfy both memory_invariant and env_lt at the same time, rather than
+    build generators separately for each. This is because of efficiency. 
+  *)
+Definition memory_invariant_bundle_with_env_lt
+           (vars: list id) (g: ctxt) (e: env) (m: memory) (st: Imp.state)
+           (bound : int) :=
+  memory_invariant g e m st
+  /\ (forall x, List.In x vars <-> exists v, g x = Some v)
+  /\ env_lt bound e.
 
-Definition aexp_correct_relation2
-           (vars : list id) (g : ctxt) (e: env) (st : Imp.state) 
-           (bound : int) (v : Ollvm_ast.value) (ans : int64)
-           (k : stack) (fn : function_id) (bid : block_id)
-           (phis : list (local_id * phi)) (term : (instr_id * terminator))
-           (s : SS.state) (mem : memory) :=
-  let '(pc', e', k') := s in  
-  satisfies_memory_invariant_and_bound (vars, g, e', mem, st) bound.
+Existing Instance gen_small_nonneg_i64.
+
+Instance gen_memory_bundle_with_env_lt (bound : int):
+  GenSizedSuchThat
+    (list id * ctxt * env * memory * Imp.state)
+    (fun '(vars, g, e, m, st) => 
+       memory_invariant_bundle_with_env_lt vars g e m st bound) :=
+  {| arbitrarySizeST :=
+       fix gen_mem n :=
+         match n with
+         | 0 => returnGen (Some ([], empty, [], [], empty_state))
+         | S n' => (* local (lid_of_Z n) *)
+           do! m_opt <- gen_mem n';
+           match m_opt with
+           | Some (idents, c, e, m, s) => 
+             do! ident <- arbitrary;
+             do! label_id <- arbitrary;
+             do! contents <- arbitrary;
+             let addr := n in (* deterministic, always appending *)
+             let label_id := if (label_id <? bound)%Z then label_id
+                             else (bound - 1)%Z in
+             let idents' := ident :: idents in
+             let c' := update c ident (local (lid_of_Z label_id)) in
+             let e' := add_env_Z label_id (DVALUE_Addr addr) e in
+             let m' := m ++ [DVALUE_I64 contents] in
+             let s' := t_update s ident contents in
+             returnGen (Some (idents', c', e', m', s'))
+           | None => returnGen None
+           end
+         end
+  |}.
+
+Remove Hints gen_small_nonneg_i64.
 
 Definition get_compiled_prefix `{eq_dec A} (code_before code_after : list A) :=
   let fix get_suffix l1 l2 :=
@@ -175,7 +191,7 @@ Definition get_compiled_prefix `{eq_dec A} (code_before code_after : list A) :=
      | None => None
      end.
 
-Fixpoint compiled_code_of (elts : list elt) :=
+Fixpoint compiled_code_of (elts : list elt) : option code :=
   match elts with
   | [] => Some []
   | I id instr :: tl =>
@@ -186,46 +202,261 @@ Fixpoint compiled_code_of (elts : list elt) :=
   | _ => None
   end.
 
-Definition empty_cfg : cfg :=
-  {| init := Name "start" ; blks := (fun blk => None); glbl := [] |}.
+Definition inject_into_tle (blocks: list Ollvm_ast.block) :
+  list (toplevel_entity (list Ollvm_ast.block)) :=
+  [
+    TLE_Definition
+      {|
+        df_prototype := imp_decl;
+        df_args := [];
+        df_instrs := blocks
+      |}
+  ].
 
+Definition build_mcfg_from_blocks (blocks: list Ollvm_ast.block) :=
+  let tle_entities := inject_into_tle blocks in
+  let m := modul_of_toplevel_entities tle_entities in
+  mcfg_of_modul m.
 
-(***************** Goals: *************************************************************
-Lemma compile_aexp_correct :
-  forall 
-    (a:aexp) (st:Imp.state) (ans:int64)
-    (HAexp: aeval st a = ans)
+Fixpoint wrap_elts_in_cfg
+         (e : list elt)
+         (instr_id_after_compiling_e : int) : err (option mcfg) :=
+  let bid := Anon 0%Z in
+  'blocks <- blocks_of_elts bid e
+          (IVoid instr_id_after_compiling_e, TERM_Ret_void);
+  mret (build_mcfg_from_blocks blocks).
 
-    (g:ctxt)
-    (n m:int) (cd:list elt)
-    (n' m':int) (cd':list elt)
-    (v : Ollvm_ast.value)
-    (Hcomp : compile_aexp g a (n,m,cd) = ((n',m',cd'),inr v)),
+(** ** Checkers *)
 
-  exists cd_a c_a,
-    cd' = cd_a ++ cd
-    /\ compiled_code cd_a c_a
-    /\ straight c_a
-    /\ forall
-    (e:env)
-    (mem:memory) (Hlt:env_lt n e)
-    (HM: memory_invariant g e mem st)
-    (k:stack)
-    (CFG : mcfg) (fn : function_id) (bid: block_id) phis term,
-      step_code
-        CFG
-        (fun s' mem' =>
-           let '(pc', e', k') := s' in
-           pc' = slc_pc fn bid phis term [] /\
-           memory_invariant g e' mem' st /\
-           Rv64e (eval_op e' (Some (TYPE_I 64)) v) ans /\
-           env_extends e e' /\
-           env_lt n' e'
-        )
-        (List.rev c_a)
-        (slc_pc fn bid phis term (List.rev c_a), e, k) mem.
+(** Given a complicated formula or property of interest, we can break it down
+    and have separate Checkers for each part. So far, we have mostly defined 
+    boolean tests, and then wrapped them up into a final Checker when running 
+    QuickChick. However, combinators like "forAll", "conjoin" and "whenFail" 
+    lets us compose Checkers, so the boolean tests could have been Checkers 
+    themselves instead. 
+ *)
 
-Notes: 
+Definition Rv64e_checker (v_err : err dvalue) (i : int64) : Checker :=
+  match v_err with
+  | inl _ => whenFail "RV64e: err" false 
+  | inr v => 
+    match v with
+    | DVALUE_I64 i' =>
+      if i == i' then 
+        checker true
+      else
+        whenFail "RV64e: not the same integer" false
+    | _ => whenFail "RV64e: not DVALUE_I64" false
+    end
+  end.
+
+(** This departs significantly from the equivalent logical form, although the 
+    equivalence should be proven. 
+    TODO: Check equivalence!
+*)
+Fixpoint env_extends_checker (e1 e2 : env) : Checker :=
+  match e1 with
+  | [] => checker true
+  | (lid1, dval1) :: l =>
+    let is_in := List.existsb
+                   (fun '(lid2, dval2) =>
+                      if (lid1 == lid2) then
+                        if (dval1 == dval2) then true else false
+                      else false)
+                   e2 in
+    if is_in then 
+      env_extends_checker l e2
+    else whenFail "env_extends: not an extension" false
+  end.
+
+Fixpoint memory_bundle_invariant_checker (vars: list id)
+         (g : ctxt) (e : env) (m : memory) (st: Imp.state) : Checker :=
+  match vars with
+  | [] => checker true
+  | Id var :: vars' =>
+    match lookup_env e (Name var) with
+    | Some (DVALUE_Addr a) =>
+      if (List.nth_default undef m a) == DVALUE_I64 (st (Id var)) then
+        memory_bundle_invariant_checker vars' g e m st
+      else whenFail "memory_invariant: values do not agree" false 
+    | _ => whenFail "memory_invariant: var not found" false
+    end
+  end.
+
+Fixpoint env_lt_checker (bound: int) (e: env) : Checker :=
+  match e with
+  | [] => checker true
+  | (Raw n, dval) :: l =>
+    if (n <? bound)%Z then env_lt_checker bound l else
+      whenFail "env_lt: fails bound" false
+  | _ => whenFail "env_lt: env not in the right form" false
+  end.
+
+Definition memory_bundle_invariant_and_env_lt_checker
+           (vars: list id) (g : ctxt) (e : env) (m : memory) (st: Imp.state)
+           (n : int) : Checker :=
+  conjoin [memory_bundle_invariant_checker vars g e m st;
+             env_lt_checker n e].
+
+Fixpoint compiled_code_checker elts code : Checker :=
+  match elts, code with
+  | [], [] => checker true
+  | (I id instr :: tl), ((id', instr') :: cd)  =>
+    if id == id' then
+      if instr == instr' then
+        compiled_code_checker tl cd
+      else whenFail "compiled_code: instrs are not equal" false
+    else whenFail "compiled_code: ids are not equal" false
+  | [], _
+  | (_ :: _), [] => whenFail "compiled_code: lengths not equal" false                     
+  | _, (_ :: _) =>
+    whenFail "compiled_code: elts not in the right form" false
+  end.
+
+Fixpoint CFG_has_code_at_checker
+         (CFG : mcfg) (P : pc -> Checker) (p : pc) (c : code) : Checker :=
+  let step_checker c_iid c_instr := 
+      match fetch CFG p with
+      | Some (CFG.Step instr) =>
+        if instr == c_instr then          
+          if (pt p == c_iid) then checker true
+          else whenFail "CFG_has_code_at: pc not in sync" false
+        else whenFail "CFG_has_code_at: instrs not the same" false
+      | Some _ => whenFail "CFG_has_code_at: jump is unexpected" false
+      | None => whenFail "CFG_has_code_at: no instruction at pc" false
+      end in
+  match c with
+  | [(iid, instr0)] =>
+    match incr_pc CFG p with
+    | Some pc_next =>
+      conjoin [step_checker iid instr0 ;
+                 whenFail "CFG_has_code_at: P does not hold for next pc"
+                          (P pc_next)]
+    | None => whenFail "CFG_has_code_at: no next pc" false
+    end
+  | (iid, instr0) :: cd =>
+    match incr_pc CFG p with
+    | Some pc_next =>
+      conjoin [step_checker iid instr0 ;
+                 CFG_has_code_at_checker CFG P pc_next cd]
+    | None => whenFail "CFG_has_code_at: no next pc" false
+    end
+  | _ => whenFail "CFG_has_code_at: code is empty, not allowed" false
+  end.
+
+Definition combine_if_then_else
+           (if_checker: Checker)
+           (then_check : Checker)
+           (else_check: Checker) : Checker :=
+  do! if_result <- liftGen unProp if_checker;
+    let '(MkRose r _) := if_result in
+  match ok r with
+  | Some true => then_check
+  | Some false | None => else_check
+  end.
+
+Fixpoint step_star_checker (CFG: mcfg) (R: SS.state -> memory -> Checker)
+         (s : SS.state) (m : memory)
+         (fuel : nat) : Checker :=
+  match fuel with
+  | 0 => R s m
+  | S fuel' => 
+    combine_if_then_else (R s m) 
+      (checker true) (* step_zero *)      
+      (match stepD CFG s with
+       | Step s' => step_star_checker CFG R s' m fuel' (* step_tau *)
+       | Obs (Eff e) =>
+         match mem_step e m with
+         | inr (m', v, k) => step_star_checker CFG R (k v) m' fuel'
+         | inl _ => whenFail "step_star: mem_step fails" false
+         end
+       | _ => whenFail "step_star: stepD to jump is unexpected" false
+       end)
+  end.
+
+Definition compile_aexp_final_state_checker
+           (llvm_ans : Ollvm_ast.value) (ans: Int64.int)           
+           (vars: list id) (g : ctxt) (e: env) (st : Imp.state)
+           (end_local_id : int) (end_pc : pc) :
+  SS.state -> memory -> Checker :=
+  fun '(pc', e', k') mem' =>
+    if pc' == end_pc then 
+    conjoin [memory_bundle_invariant_checker vars g e' mem' st ;
+               Rv64e_checker (eval_op e (Some (TYPE_I 64)%Z) llvm_ans) ans;
+               env_extends_checker e e';
+               env_lt_checker end_local_id e']
+    else whenFail "compile_aexp: final state has wrong pc" false.
+
+Definition unsafe_aexp_compiled_code_checker
+           (llvm_ans: Ollvm_ast.value) (ans: int64)
+           (end_local_id : int)
+           (vars: list id) (g: ctxt) (e: env) (m: memory) (st: Imp.state)
+           (CFG: mcfg) (start_pc: pc) (k: stack) (end_pc: pc)
+           (c : code) : Checker :=
+  match c with
+  | [] => Rv64e_checker (eval_op e (Some (TYPE_I 64)%Z) llvm_ans) ans
+  | _ :: _ =>
+    step_star_checker CFG
+                      (compile_aexp_final_state_checker
+                         llvm_ans ans
+                         vars g e st
+                         end_local_id end_pc)
+                      (start_pc, e, k) m 1000
+  end.
+
+(*! Section TestCompileAexp *)
+
+(** Hiccups: Typeclass magic means that subtle mistakes can make the typechecker
+    run forever. 
+    (1) Try interchanging arguments for memory_invariant_bundle_with_env_lt.
+    (2) Partial-evaluate whenFail, i.e. without false, say.
+ *)
+
+Existing Instance gen_small_nonneg_i64.
+Existing Instance genSaexp.
+
+Definition check_compile_aexp_correct_simple : Checker := 
+  forAll arbitrary (fun (a : aexp) =>
+  forAll arbitrary (fun (local_id instr_id : int) =>
+  forAll arbitrary (fun (cd : list elt) => 
+  forAll (genST (fun '(vars, g, e, m, st) =>
+               memory_invariant_bundle_with_env_lt vars g e m st local_id))
+  (fun bundled_memory_opt =>
+     match bundled_memory_opt with
+     | None => whenFail "generation of compatible memory failed" false
+     | Some (vars, g, e, m, st) =>
+       forAll arbitrary (fun (k : stack) => 
+       let ans := aeval st a in
+       let '((n', m', cd'), v_opt) :=
+           compile_aexp g a (local_id, instr_id, cd) in
+       match v_opt with
+       | inl _ => whenFail "compilation failed" true
+       | inr v =>
+         match get_compiled_prefix cd cd' with
+         | Some cd_a => 
+           match compiled_code_of cd_a with
+           | Some c_a =>
+             match wrap_elts_in_cfg (List.rev cd_a) m' with
+             | inr cfg =>
+               checker true
+               (* unsafe_aexp_compiled_code_checker v ans n'
+                                                 vars g e m st
+                                                 cfg m k m' (List.rev c_a)
+                *)
+             | inl _ => whenFail "CFG generation failed" false
+             end
+           | None => whenFail "compiled code not well-formed" false
+           end
+         | None => whenFail "compiled code not prefix" false
+         end
+       end)
+     end)))). 
+
+(*! QuickChick check_compile_aexp_correct_simple. *)
+
+(* End TestCompileAexp *)
+
+(** ** Notes *******************************************************************
 - Prenexification
 - Functional dependence of exists
 - Further constraints after exists
@@ -235,67 +466,6 @@ Notes:
   so that both generation and testing use one copy. 
 - Higher-order constructs are difficult, e.g. continuation for effects and
   partial maps for Imp.state. 
-
-Lemma compile_aexp_correct_simple1:
-  forall (a : aexp) (st : Imp.state) (g : ctxt)
-    (e : env) (mem : memory) (vars : list id)
-    (n m : int) (cd : list elt)
-    (n' m' : int) (cd' : list elt) (v_err : err Ollvm_ast.value),
-    (* Simplification: restriction to compatible e, m *) 
-    satisfies_memory_invariant_and_bound (vars, g, e, mem, st) n /\
-    compile_aexp g a (n, m, cd) = ((n', m', cd'), v_err) ->
-    match v_err with
-    | inl err => True (* Says nothing *)
-    | inr v =>       
-      let cd_a := get_compiled_prefix cd cd' in
-      match cd_a with
-      | None => False
-      | Some cd_a =>
-        let c_a := compiled_code_of cd_a in
-        match c_a with
-        | None => False
-        | Some c_a => 
-          (forall (k : stack) (CFG: mcfg) (fn : function_id) (bid: block_id) phis term,
-              step_code CFG
-                        (aexp_correct_relation1 vars g e st n' v
-                                                (aeval st a)
-                                                k fn bid phis term)
-                        (List.rev c_a)
-                        (slc_pc fn bid phis term c_a, e, k)
-                        mem)
-        end
-      end
-    end.
-
-Lemma compile_aexp_correct_simple2:
-  forall (a : aexp) (st : Imp.state) (g : ctxt)
-    (e : env) (mem : memory) (vars : list id)
-    (n m : int) (cd : list elt)
-    (n' m' : int) (cd' : list elt) (v_err : err Ollvm_ast.value),
-    satisfies_memory_invariant_and_bound (vars, g, e, mem, st) n /\
-    compile_aexp g a (n, m, cd) = ((n', m', cd'), v_err) ->
-    match v_err with
-    | inl err => True (* Says nothing *)
-    | inr v =>       
-      let cd_a := get_compiled_prefix cd cd' in
-      match cd_a with
-      | None => False
-      | Some cd_a =>
-        let c_a := compiled_code_of cd_a in
-        match c_a with
-        | None => False
-        | Some c_a => 
-          (forall (k : stack) (CFG: mcfg) (fn : function_id) (bid: block_id) phis term,
-              step_code CFG
-                        (aexp_correct_relation2 vars g e st n' v
-                                                (aeval st a)
-                                                k fn bid phis term)
-                        (List.rev c_a)
-                        (slc_pc fn bid phis term c_a, e, k)
-                        mem)
-        end
-      end
-    end.
 
 Lemma compile_aexp_correct_simple2A:
   forall (a : aexp) (st : Imp.state) (g : ctxt)
@@ -325,49 +495,50 @@ Lemma compile_aexp_correct_simple2A:
         end
       end
     end.
-****)
 
-Definition aexp_correct_relation_bool2
-           (vars : list id) (g : ctxt) (e: env) (st : Imp.state) 
-           (bound : int) (v : Ollvm_ast.value) (ans : int64)
-           (k : stack) (fn : function_id) (bid : block_id)
-           (phis : list (local_id * phi)) (term : (instr_id * terminator))
-           (s : SS.state) (mem : memory) : bool :=
-  let '(pc', e', k') := s in  
-  check_memory_invariant_and_bound (vars, g, e', mem, st) bound.
-
-Definition inject_into_tle elts :=
-  'blocks <- blocks_of_elts (Anon 0)%Z elts;
-    mret
-   ([
-    TLE_Definition
-    {|
-    df_prototype := imp_decl;
-    df_args := [];
-    df_instrs := blocks
-    |}]).
-
-Definition build_mcfg elts :=
-  match inject_into_tle elts with
-  | inl err => None
-  | inr entities => 
-    let m := modul_of_toplevel_entities entities in
-    mcfg_of_modul m
-  end.
-
-Instance dec_is_Op : forall (i : instr), Decidable (is_Op i).
-Proof.
-  intros i; unfold Decidable; destruct i;
-    try solve [right; intros H; inversion H; auto];
-    try solve [left; constructor].
-Defined.
-
-Instance dec_is_Eff : forall (i : instr), Decidable (is_Eff i).
-Proof.
-  intros i; unfold Decidable; destruct i;
-    try solve [right; intros H; inversion H; auto];
-    try solve [left; constructor].
-Defined.
+Definition check_compile_aexp_correct_simple2A :=
+  forAll arbitrary
+         (fun (a : aexp) => 
+         forAll (genST (fun bundle => satisfies_memory_invariant_and_bound bundle 0)%Z)
+         (fun bundle =>
+            match bundle with
+            | None => checker true
+            | Some (vars, g, e, mem, st) =>
+              let result := compile_aexp g a (0, 0, [])%Z in
+              match result with
+              | ((n', m', cd'), inr v) =>
+                let cd_a := get_compiled_prefix [] cd' in
+                match cd_a with
+                | None => whenFail "not monotonic" false
+                | Some cd_a =>
+                  let c_a := compiled_code_of cd_a in
+                  match c_a with
+                  | None => whenFail "compiled result not well-formed" false
+                  | Some c_a =>
+                    match build_mcfg cd_a with
+                    | None => checker true
+                    | Some mcfg =>
+                      forAll arbitrary
+                             (fun (k : stack) => forAll arbitrary
+                             (fun (fn : function_id) => forAll arbitrary
+                             (fun (bid : block_id) => forAll arbitrary
+                             (fun phis => forAll arbitrary
+                             (fun term =>
+                                step_code_bool
+                                  mcfg
+                                  (aexp_correct_relation_bool2 vars g e st n' v
+                                                               (aeval st a)
+                                                               k fn bid phis term)
+                                  (List.rev c_a)
+                                  (slc_pc fn bid phis term c_a, e, k)
+                                  mem)))))
+                    end
+                  end
+                end
+              | _ => whenFail "couldn't compile" true
+              end
+            end)).
+*)
 
 (*
 Instance dec_stepD_is_Step : forall CFG (s s' : SS.state), Decidable (stepD CFG s = Step s').
@@ -446,143 +617,47 @@ Proof.
     { destruct i0.
 *)
 
-Fixpoint step_code_bool (CFG : mcfg) (R : SS.state -> memory -> bool)
-         (cs : code) (st : SS.state) (mem : memory) : bool :=
-  match cs, st, mem with
-  | [], s, m => if R s m then true else false
-  | (id, i) :: cd, s, m =>
-    if decide (is_Op i) then
-      (* missing prefix test *)
-      match stepD CFG s with
-      | Step s' => step_code_bool CFG R cd s' m
-      | _ => false
-      end
-    else
-      if decide (is_Eff i) then
-        (* missing prefix test *)
-        match stepD CFG s with
-        | Obs (Eff e) =>
-          match mem_step e m with
-          | inr (m', v, k) =>
-            step_code_bool CFG R cd (k v) m'
-          | inl _ => false
-          end
-        | _ => false
-        end
-      else true
-  end.
 
-Existing Instance gen_adhoc_aexp.
 
-Instance show_bundled_memory : Show bundled_memory :=
-  {| show x := 
-       match x with
-       | (ids, c, e, m, s) =>
-         ("vars: " ++ (show ids) ++ "; " ++
-                   "env: " ++ (show e) ++ "; " ++
-                   "mem: " ++ (show m) ++ "; ")%string
-       end
-  |}.
-
-Instance gen_consistent_memory (bound : int):
-  GenSizedSuchThat bundled_memory (fun m => satisfies_memory_invariant_and_bound m bound) :=
-  {| arbitrarySizeST :=
-       fix gen_mem n :=
-         match n with
-         | 0 => returnGen (Some ([], empty, [], [], empty_state))
-         | S n' => (* local (lid_of_Z n) *)
-           do! m_opt <- gen_mem n';
-           match m_opt with
-           | Some (idents, c, e, m, s) => 
-             do! ident <- arbitrary;
-             do! label_id <- arbitrary;
-             do! contents <- arbitrary;
-             let addr := n in (* deterministic, always appending *)
-             let label_id := if Z.leb bound label_id then bound else label_id in
-             let idents' := ident :: idents in
-             let c' := update c ident (local (lid_of_Z label_id)) in
-             let e' := add_env_Z label_id (DVALUE_Addr addr) e in
-             let m' := m ++ [DVALUE_I64 contents] in
-             let s' := t_update s ident contents in
-             returnGen (Some (idents', c', e', m', s'))
-           | None => returnGen None
-           end
-         end
-  |}.
-
-Definition check_compile_aexp_correct_simple2A :=
-  forAll arbitrary
-         (fun (a : aexp) => 
-         forAll (genST (fun bundle => satisfies_memory_invariant_and_bound bundle 0)%Z)
-         (fun bundle =>
-            match bundle with
-            | None => checker true
-            | Some (vars, g, e, mem, st) =>
-              let result := compile_aexp g a (0, 0, [])%Z in
-              match result with
-              | ((n', m', cd'), inr v) =>
-                let cd_a := get_compiled_prefix [] cd' in
-                match cd_a with
-                | None => whenFail "not monotonic" false
-                | Some cd_a =>
-                  let c_a := compiled_code_of cd_a in
-                  match c_a with
-                  | None => whenFail "compiled result not well-formed" false
-                  | Some c_a =>
-                    match build_mcfg cd_a with
-                    | None => checker true
-                    | Some mcfg =>
-                      forAll arbitrary
-                             (fun (k : stack) => forAll arbitrary
-                             (fun (fn : function_id) => forAll arbitrary
-                             (fun (bid : block_id) => forAll arbitrary
-                             (fun phis => forAll arbitrary
-                             (fun term =>
-                                step_code_bool
-                                  mcfg
-                                  (aexp_correct_relation_bool2 vars g e st n' v
-                                                               (aeval st a)
-                                                               k fn bid phis term)
-                                  (List.rev c_a)
-                                  (slc_pc fn bid phis term c_a, e, k)
-                                  mem)))))
-                    end
-                  end
-                end
-              | _ => whenFail "couldn't compile" true
-              end
-            end)).
-
-(*! QuickChick check_compile_aexp_correct_simple2A. *)
-
-Instance show_mcfg : Show mcfg := {| show x := "(show mcfg not implemented)" |}.
-
-(*
-Definition is_env_extends (e e' : env) : Decidable (env_extends e e').
-Proof.
-  induction e; unfold Decidable.
-  - left. unfold env_extends.
-    intros op t dv eval_op_empty.
-    destruct op; destruct e; inversion eval_op_empty.
-    destruct t; simpl in *.
-   ;
-    
-  match e with
-  | [] => inl _
-  | [] => 
+(** ** Sidetrack into verified generators *)
+(** The generators for propositions above are entirely unchecked and trusted to 
+    be generating the right elements, but this may not be true as code and 
+    logical definitions evolve. To keep test suites in sync with the 
+    development, it can be useful to go the extra mile and prove generators
+    "correct".
 *)
+Instance gen_aevalR (st : Imp.state) (a : aexp) :
+  GenSuchThat Int64.int (fun ans => aevalR st a ans) :=
+  {| arbitraryST := returnGen (Some (aeval st a)) |}.
 
-Derive ArbitrarySizedSuchThat for (fun (instr : instr) => is_Op instr).
-Derive ArbitrarySizedSuchThat for (fun (instr : instr) => is_Eff instr).
+Instance gen_aevalR_is_correct (st: Imp.state) (a : aexp) :
+  SuchThatCorrect (fun ans => aevalR st a ans) (genST (fun ans => aevalR st a ans)).
+Proof.
+  unfold arbitraryST; simpl.
+  constructor; rewrite semReturn; 
+    unfold Sets.lift, imset, set_incl, bigcup, set1, setU.
+  - intros a' [ans (H_eval_to_ans, H_some_ans)].
+    rewrite <- aeval_iff_aevalR in H_eval_to_ans.
+    rewrite H_eval_to_ans; auto.
+  - intros [a' | ] H_aeval; try solve [right; inversion H_aeval].
+    left; exists a'; split; auto.
+    rewrite <- aeval_iff_aevalR.
+    inversion H_aeval; trivial.
+Qed.
 
-(* 
+Instance gen_aevalR_correct (st: Imp.state) (a:aexp):
+  GenSuchThatCorrect (fun ans: Int64.int => aevalR st a ans).
+
+(** The generator is actually redundant, because it is just running a function;
+    it makes better sense to run the function directly and not sample at all. 
+    But this shows how we can use an algorithm corresponding to a predicate as 
+    a generator for it, and to also use its equivalence proof to prove the 
+    generator correct. Verified testing keeps it in sync with code changes and 
+    proofs. *)
+
+(** ** Junk ********************************************************************
 QuickChickDebug Debug On. 
 Print GenSizedSuchThatis_Op.
-Print Hint GenSizedSuchThat. 
-Sample (@arbitraryST instr (fun instr => is_Op instr) _).
-*)
-
-(* Derive ArbitrarySizedSuchThat for (fun code => straight code)). *)
 
 Instance gen_straight_code : GenSizedSuchThat code (fun c => straight c) :=
   {| arbitrarySizeST :=
@@ -597,128 +672,18 @@ Instance gen_straight_code : GenSizedSuchThat code (fun c => straight c) :=
          end
   |}.
 
-Fixpoint is_Op_bool (i : instr) : bool :=
-  match i with
-  | INSTR_Op _ => true
-  | _ => false
-  end.
-
-Fixpoint is_Eff_bool (i : instr) : bool :=
-  match i with
-  | INSTR_Alloca _ _ _ => true
-  | INSTR_Load _ _ _ _ => true
-  | INSTR_Store _ _ _ _ => true
-  | _ => false
-  end.
-
-Fixpoint straight_bool (c : code) : bool :=
-  match c with
-  | [] => true
-  | ((id, i) :: c') =>
-    if orb (is_Op_bool i) (is_Eff_bool i) then straight_bool c'
-    else false
-  end.
-
-Fixpoint compiled_code_bool elts code : bool :=
-  match elts, code with
-  | [], [] => true
-  | (I id instr :: tl), ((id', instr') :: cd)  =>
-    if id == id' then
-      if instr == instr' then
-        compiled_code_bool tl cd
-      else false
-    else false
-  | _, _ => false
-  end.
-
-(* Derive ArbitrarySizedSuchThat for (fun env => env_lt n env). *)
-
-Instance gen_env_lt (bound : int) :
-  GenSizedSuchThat env (fun env => env_lt bound env) :=
-  
-  {| arbitrarySizeST :=
-       fix gen_env_lt n :=
-         match n with
-         | 0 => returnGen (Some [])
-         | S n' =>
-           do! n <- arbitrary;
-           do! dv <- arbitrary;
-           let m := if Z.leb bound n then bound else n in
-           do! env_opt <- gen_env_lt n';
-           match env_opt with
-           | Some env' =>
-             returnGen (Some (add_env_Z m dv env'))
-           | None =>
-             returnGen None
-           end
-         end
-  |}.
-
-
-(* 
-Sample (genST (fun m => satisfies_memory_invariant_and_bound m 3)%Z).
-Sample (@arbitrary stack _) 
-Sample (@arbitrary function_id _).
-Sample (@arbitrary block_id _).
-Sample (@arbitrary instr_id _).
-Sample (@arbitrary phi _).
-Sample (@arbitrary terminator _).
-Sample (@arbitrary code _).
- *)
-
-(*
-Definition check_compile_aexp_correct :=
-  forAll arbitrary
-         (fun (a : aexp) => forAll arbitrary
-         (fun (st : Imp.state) =>
-         forAll (genST (fun bundle => satisfies_memory_invariant_and_bound bundle 3)%Z)
-         (fun bundle =>
-            match bundle with
-            | None => checker true
-            | Some (vars, g, env, mem, state) =>
-              let result := compile_aexp g a (0, 0, [])%Z in
-              match result with
-              | ((n', m', cd'), inr v) =>
-                forAll arbitrary
-                       (fun (k : stack) => forAll arbitrary
-                       (* (fun (CFG : mcfg) => forAll arbitrary *)
-                       (fun (fn : function_id) => forAll arbitrary
-                       (fun (bid : block_id) => forAll arbitrary
-                       (fun phis => forAll arbitrary
-                       (fun term =>
-                          step_code_checker
-                            CFG
-                            (fun s' mem' =>
-                               let '(pc', e', k') := s' in
-                               (* pc' == slc_pc fn bid phis term [] *)
-                               check_memory_invariant_and_bound (, g, e', mem', ) n'
-                       )))))
-              | _ => checker false
-              end
-                        end))).
-*)
-          
-
-(*
 Inductive fooP : nat -> Foo -> Prop.
 Instance dec_dooP n : Dec (foo n).
 
 if (fooP 42)? then ...
 else ...
 
-pp
-*)
-
-(*
 From QuickChick Require Import QuickChick.
 Local Open Scope nat.
 Import Ollvm_ast.
 Derive Arbitrary for Expr
 Derive Arbitrary for value.
-
 *)
 
-(* Derive ArbitrarySizedSuchThat for (fun env => env_lt n env). *)
-(* Sample (genST (fun env => env_tl env)). *)
 
-(* Derive ArbitrarySizedSuchThat for (fun instr => is_Op instr). *)
+    
